progress with merkel tree

theories/ub_logic/merkel_tree.v
@@ -1,3 +1,110 @@
-From clutch.ub_logic Require Export ub_clutch lib.map hash.
+From clutch.ub_logic Require Export ub_clutch lib.map hash lib.list.
 Import Hierarchy.
 Set Default Proof Using "Type*".
+
+Section merkel_tree.
+  Context `{!ub_clutchGS Σ}.
+  Variables height:nat.
+  Variables val_bit_size':nat.
+  Variables max_hash_size : nat.
+  Definition val_bit_size : nat := S val_bit_size'.
+  Definition val_size:nat := (2^val_bit_size)-1.
+  Variable (Hineq: (max_hash_size <= val_size)%nat).
+  Definition leaf_bit_size : nat := 2*val_bit_size.
+  (* Definition identifier : nat := 2^leaf_bit_size. *)
+  Definition num_of_leafs : nat := 2^height.
+  
+  Inductive merkel_tree :=
+  | Leaf (hash_value : nat) (leaf_value:nat)
+  | Branch (hash_value : nat) (t1 t2:merkel_tree).
+
+  Definition root_hash_value (t: merkel_tree) :=
+    match t with
+    | Leaf h _ => h
+    | Branch h _ _ => h
+    end.
+    
+  Fixpoint tree_relate (h:nat) (lt : val) (t:merkel_tree) : Prop:=
+    match h with
+    |0 => (∃ (hv v:nat), lt = InjLV (#hv, #v) /\ t = Leaf hv v)
+    |S h' => ∃ (hv:nat) (ll lr:val) (l r:merkel_tree), lt = InjRV (#hv, ll, lr) /\ t = Branch hv l r /\
+                                tree_relate h' ll l /\ tree_relate h' lr r 
+  end.
+
+  Fixpoint tree_valid (t:merkel_tree) (m:gmap nat Z) : Prop :=
+    match t with
+    | Leaf h l => h < 2^val_bit_size /\ l < 2^leaf_bit_size /\ m!!l%nat = Some (Z.of_nat h)
+    | Branch h l r => h < 2^val_bit_size /\ m!!((root_hash_value l)*2^val_bit_size + root_hash_value r)%nat=Some (Z.of_nat h) /\ tree_valid l m /\ tree_valid r m
+    end.
+
+  Definition map_valid (m:gmap nat Z) : Prop := coll_free m.
+
+  Definition compute_hash_from_leaf : val :=
+    rec: "compute_hash_from_leaf" "ltree" "lhmf" "ll" "lf" := 
+    match: "ltree" with
+    | InjL "x" => "lhmf" "lf"  
+    | InjR "x"  => let: "b" := (match: list_head "ll" with
+                               | SOME "a" => "a"
+                               | NONE => #()
+                               end
+                              ) in
+                  let: "ll'" := (match: list_tail "ll" with
+                               | SOME "a" => "a"
+                               | NONE => #()
+                                 end
+                                ) in
+                  let, ("l", "r") := Snd "x" in
+                  if: "b"
+                  then "lhmf"
+                         (("compute_hash_from_leaf" "l" "lhmf" "ll'" "lleaf")*#(2^val_bit_size)+"r")
+                  else "lhmf"
+                         ("l"*#(2^val_bit_size)+("compute_hash_from_leaf" "r" "lhmf" "ll'" "lleaf"))
+    end
+
+  .
+
+   Fixpoint tree_value_match (tree:merkel_tree) (v:nat) (path:list bool) :=
+     match (tree, path) with
+     | (Leaf h lf, []) => lf=v
+     | (Branch h l r, x::xs) => if x then tree_value_match l v xs else tree_value_match r v xs
+     | _ => False
+     end.
+
+  (** Lemmas *)
+  Lemma tree_relate_leaf h ltree a b :
+    tree_relate h ltree (Leaf a b) -> h = 0%nat /\ ltree = InjLV (#a, #b).
+  Proof.
+  Admitted.
+  
+
+  (** Spec *)
+  Lemma wp_correct_check (ltree:val) (tree:merkel_tree) (m:gmap nat Z) (v:nat) (path:list bool) llist f E:
+     {{{ ⌜tree_relate height ltree tree⌝ ∗
+        ⌜tree_valid tree m⌝ ∗
+        hashfun_amortized (val_size-1)%nat max_hash_size f m ∗
+        ⌜is_list path llist⌝ ∗
+        ⌜tree_value_match tree v path⌝ ∗
+        ⌜map_valid m⌝ }}}
+      compute_hash_from_leaf ltree f llist (#v) @ E
+      {{{ (retv:Z), RET #retv;
+          hashfun_amortized (val_size-1) max_hash_size f m ∗
+          ⌜retv = root_hash_value tree⌝
+      }}}.
+  Proof.
+    iIntros (Φ) "(%Htrelate&%Htvalid&H&%Hlsit&%Hvmatch&%Hmvalid) HΦ".
+    revert Htrelate Htvalid Hlsit Hvmatch Hmvalid.
+    revert height ltree v path llist f.
+    induction tree.
+    - intros.
+      rewrite /compute_hash_from_leaf.
+      wp_pures. apply tree_relate_leaf in Htrelate as [-> ->].
+      wp_match.
+      wp_apply (wp_hashfun_prev_amortized with "[$]").
+      + lia.
+      + admit.
+      + admit.
+      
+    - admit.
+  Admitted.
+  
+End merkel_tree.
